A little tidying

thys/Jinja/BV/BVExample.thy
@@ -480,19 +480,7 @@ lemma [code]:
    fold (\<lambda>p A. if \<not>stable r step ss p then insert p A else A) [0..<size ss] {}"
 proof -
   have "unstables r step ss = (UN p:{..<size ss}. if \<not>stable r step ss p then {p} else {})"
-    apply (unfold unstables_def)
-    apply (rule equalityI)
-    apply (rule subsetI)
-    apply (erule CollectE)
-    apply (erule conjE)
-    apply (rule UN_I)
-    apply simp
-    apply simp
-    apply (rule subsetI)
-    apply (erule UN_E)
-    apply (case_tac "\<not> stable r step ss p")
-    apply simp+
-    done
+    by (auto simp: unstables_def)
   also have "\<And>f. (UN p:{..<size ss}. f p) = Union (set (map f [0..<size ss]))" by auto
   also note Sup_set_fold also note fold_map
   also have "(\<union>) \<circ> (\<lambda>p. if \<not> stable r step ss p then {p} else {}) = 
@@ -501,8 +489,7 @@ proof -
   finally show ?thesis .
 qed
 
-definition some_elem :: "'a set \<Rightarrow> 'a" where [code del]:
-  "some_elem = (%S. SOME x. x : S)"
+declare some_elem_def [code del]
 code_printing
   constant some_elem \<rightharpoonup> (SML) "(case/ _ of/ Set/ xs/ =>/ hd/ xs)"
 
@@ -524,10 +511,9 @@ lemma JVM_sup_unfold [code]:
  "JVM_SemiType.sup S m n = lift2 (Opt.sup
        (Product.sup (Listn.sup (SemiType.sup S))
          (\<lambda>x y. OK (map2 (lift2 (SemiType.sup S)) x y))))" 
-  apply (unfold JVM_SemiType.sup_def JVM_SemiType.sl_def Opt.esl_def Err.sl_def
+  by (auto simp: JVM_SemiType.sup_def JVM_SemiType.sl_def Opt.esl_def Err.sl_def
          stk_esl_def loc_sl_def Product.esl_def  
          Listn.sl_def upto_esl_def SemiType.esl_def Err.esl_def)
-  by simp
 
 lemmas [code] = SemiType.sup_def [unfolded exec_lub_def] JVM_le_unfold
 
